LinearScan/IState.hs
@@ -5,6 +5,7 @@ module LinearScan.IState where
 
 import qualified Prelude
 import qualified Data.List
+import qualified Data.Ord
 import qualified Data.Functor.Identity
 import qualified LinearScan.Utils
 import qualified LinearScan.IApplicative as IApplicative
