LinearScan/Interval.hs
@@ -5,11 +5,11 @@ module LinearScan.Interval where
 
 import qualified Prelude
 import qualified Data.List
+import qualified Data.Ord
 import qualified Data.Functor.Identity
 import qualified LinearScan.Utils
 import qualified LinearScan.Lib as Lib
 import qualified LinearScan.Logic as Logic
-import qualified LinearScan.NonEmpty0 as NonEmpty0
 import qualified LinearScan.Range as Range
 import qualified LinearScan.Eqtype as Eqtype
 import qualified LinearScan.Ssrnat as Ssrnat
@@ -30,8 +30,7 @@ __ :: any
 __ = Prelude.error "Logical or arity value used"
 
 data IntervalDesc =
-   Build_IntervalDesc Prelude.Int Prelude.Int (NonEmpty0.NonEmpty
-                                              Range.RangeDesc)
+   Build_IntervalDesc Prelude.Int Prelude.Int ([] Range.RangeDesc)
 
 ibeg :: IntervalDesc -> Prelude.Int
 ibeg i =
@@ -43,7 +42,7 @@ iend i =
   case i of {
    Build_IntervalDesc ibeg0 iend0 rds0 -> iend0}
 
-rds :: IntervalDesc -> NonEmpty0.NonEmpty Range.RangeDesc
+rds :: IntervalDesc -> [] Range.RangeDesc
 rds i =
   case i of {
    Build_IntervalDesc ibeg0 iend0 rds0 -> rds0}
@@ -72,34 +71,29 @@ intervalExtent d =
 coq_Interval_is_singleton :: IntervalDesc -> Prelude.Bool
 coq_Interval_is_singleton d =
   (Prelude.&&)
-    (Eqtype.eq_op Ssrnat.nat_eqType
-      (unsafeCoerce (NonEmpty0.coq_NE_length (rds d)))
+    (Eqtype.eq_op Ssrnat.nat_eqType (unsafeCoerce (Prelude.length (rds d)))
       (unsafeCoerce ((Prelude.succ) 0)))
     (Eqtype.eq_op Ssrnat.nat_eqType
-      (unsafeCoerce
-        (NonEmpty0.coq_NE_length
-          (Range.ups ( (NonEmpty0.coq_NE_head (rds d))))))
+      (unsafeCoerce (Prelude.length (Range.ups ( (Prelude.head (rds d))))))
       (unsafeCoerce ((Prelude.succ) 0)))
 
 intervalsIntersect :: IntervalDesc -> IntervalDesc -> Prelude.Bool
 intervalsIntersect i j =
   let {f = \x y -> Range.rangesIntersect ( x) ( y)} in
-  Data.List.any (\x ->
-    Data.List.any (f x) (NonEmpty0.coq_NE_to_list (rds j)))
-    (NonEmpty0.coq_NE_to_list (rds i))
+  Data.List.any (\x -> Data.List.any (f x) ( (rds j))) ( (rds i))
 
 intervalIntersectionPoint :: IntervalDesc -> IntervalDesc -> Prelude.Maybe
                              Prelude.Int
 intervalIntersectionPoint i j =
-  NonEmpty0.coq_NE_fold_left (\acc rd ->
+  Data.List.foldl' (\acc rd ->
     case acc of {
      Prelude.Just x -> Prelude.Just x;
      Prelude.Nothing ->
-      NonEmpty0.coq_NE_fold_left (\acc' rd' ->
+      Data.List.foldl' (\acc' rd' ->
         case acc' of {
          Prelude.Just x -> Prelude.Just x;
          Prelude.Nothing -> Range.rangeIntersectionPoint ( rd) ( rd')})
-        (rds j) Prelude.Nothing}) (rds i) Prelude.Nothing
+        Prelude.Nothing (rds j)}) Prelude.Nothing (rds i)
 
 findIntervalUsePos :: IntervalDesc -> (Range.UsePos -> Prelude.Bool) ->
                       Prelude.Maybe ((,) Range.RangeDesc Range.UsePos)
@@ -112,9 +106,12 @@ findIntervalUsePos i f =
   in
   let {
    go rs =
-     case rs of {
-      NonEmpty0.NE_Sing r -> f0 r;
-      NonEmpty0.NE_Cons r rs' -> Lib.option_choose (f0 r) (go rs')}}
+     (\ns nc l -> case l of [x] -> ns x; (x:xs) -> nc x xs)
+       (\r ->
+       f0 r)
+       (\r rs' ->
+       Lib.option_choose (f0 r) (go rs'))
+       rs}
   in go (rds i)
 
 nextUseAfter :: IntervalDesc -> Prelude.Int -> Prelude.Maybe Prelude.Int
@@ -125,8 +122,7 @@ nextUseAfter d pos =
 
 firstUsePos :: IntervalDesc -> Prelude.Int
 firstUsePos d =
-  Range.uloc
-    (NonEmpty0.coq_NE_head (Range.ups ( (NonEmpty0.coq_NE_head (rds d)))))
+  Range.uloc (Prelude.head (Range.ups ( (Prelude.head (rds d)))))
 
 firstUseReqReg :: IntervalDesc -> Prelude.Maybe Prelude.Int
 firstUseReqReg d =
@@ -135,8 +131,7 @@ firstUseReqReg d =
 
 lastUsePos :: IntervalDesc -> Prelude.Int
 lastUsePos d =
-  Range.uloc
-    (NonEmpty0.coq_NE_last (Range.ups ( (NonEmpty0.coq_NE_last (rds d)))))
+  Range.uloc (Prelude.last (Range.ups ( (Prelude.last (rds d)))))
 
 splitPosition :: IntervalDesc -> (Prelude.Maybe Prelude.Int) -> Prelude.Bool
                  -> Prelude.Int
@@ -147,102 +142,208 @@ splitPosition d before splitBeforeLifetimeHole =
     (Prelude.min final
       (Lib.fromMaybe final (Lib.option_choose before (firstUseReqReg d))))
 
-intervalSpan_subproof :: (NonEmpty0.NonEmpty Range.RangeDesc) -> Prelude.Int
-                         -> Prelude.Int -> Prelude.Int ->
-                         ((,) (Prelude.Maybe IntervalDesc)
-                         (Prelude.Maybe IntervalDesc))
-intervalSpan_subproof rs before ib ie =
-  case rs of {
-   NonEmpty0.NE_Sing r ->
-    case Range.rangeSpan (\u ->
-           (Prelude.<=) ((Prelude.succ) (Range.uloc u)) before) ( r) of {
-     (,) _top_assumption_ x ->
-      case _top_assumption_ of {
-       Prelude.Just r0 ->
-        case x of {
-         Prelude.Just r1 ->
-          
-            ( (\_ _ -> (,) (Prelude.Just (Build_IntervalDesc
-              (Range.rbeg ( r0)) (Range.rend ( r0)) (NonEmpty0.NE_Sing
-              ( r0)))) (Prelude.Just (Build_IntervalDesc (Range.rbeg ( r1))
-              (Range.rend ( r1)) (NonEmpty0.NE_Sing ( r1)))))) __ __;
-         Prelude.Nothing ->
-           (\_ -> (,) (Prelude.Just (Build_IntervalDesc ib ie
-            (NonEmpty0.NE_Sing r))) Prelude.Nothing) __};
-       Prelude.Nothing ->
-        case x of {
-         Prelude.Just r1 ->
-           (\_ -> (,) Prelude.Nothing (Prelude.Just (Build_IntervalDesc ib ie
-            (NonEmpty0.NE_Sing r)))) __;
-         Prelude.Nothing -> Logic.coq_False_rec}}};
-   NonEmpty0.NE_Cons r rs0 ->
-    case Range.rangeSpan (\u ->
-           (Prelude.<=) ((Prelude.succ) (Range.uloc u)) before) ( r) of {
-     (,) _top_assumption_ x ->
-      case _top_assumption_ of {
-       Prelude.Just r0 ->
-        case x of {
-         Prelude.Just r1 ->
-           (\_ ->
-             (\_ _ ->
-              (Prelude.flip (Prelude.$)) __ (\_ -> (,) (Prelude.Just
-                (Build_IntervalDesc (Range.rbeg ( r0)) (Range.rend ( r0))
-                (NonEmpty0.NE_Sing ( r0)))) (Prelude.Just (Build_IntervalDesc
-                (Range.rbeg ( r1))
-                (Range.rend ( (NonEmpty0.coq_NE_last rs0)))
-                (NonEmpty0.NE_Cons r1 rs0))))) __ __) __;
-         Prelude.Nothing ->
-           (\_ ->
-             (\_ ->
-              case intervalSpan_subproof rs0 before
-                     (Range.rbeg ( (NonEmpty0.coq_NE_head rs0)))
-                     (Range.rend ( (NonEmpty0.coq_NE_last rs0))) of {
-               (,) _top_assumption_0 x0 ->
-                case _top_assumption_0 of {
-                 Prelude.Just i1_1 ->
-                  case x0 of {
-                   Prelude.Just i1_2 ->
-                    case i1_1 of {
-                     Build_IntervalDesc ibeg0 iend0 rds0 ->
-                      
-                        ( (\_ _ ->
-                           (\_ ->
-                             (\_ ->
-                              
-                                ((Prelude.flip (Prelude.$)) __ (\_ ->
-                                   (\_ _ -> (,) (Prelude.Just
-                                    (Build_IntervalDesc (Range.rbeg ( r))
-                                    iend0 (NonEmpty0.NE_Cons r rds0)))
-                                    (Prelude.Just i1_2)) __))) __) __)) __ __
-                        __};
-                   Prelude.Nothing ->
-                     (\_ _ _ -> (,) (Prelude.Just (Build_IntervalDesc
-                      (Range.rbeg ( r))
-                      (Range.rend ( (NonEmpty0.coq_NE_last rs0)))
-                      (NonEmpty0.NE_Cons r rs0))) Prelude.Nothing) __ __ __};
-                 Prelude.Nothing ->
-                  case x0 of {
-                   Prelude.Just i1_2 ->
-                     (\_ _ _ -> (,) (Prelude.Just (Build_IntervalDesc ib
-                      (Range.rend ( r)) (NonEmpty0.NE_Sing r))) (Prelude.Just
-                      (Build_IntervalDesc
-                      (Range.rbeg ( (NonEmpty0.coq_NE_head rs0)))
-                      (Range.rend ( (NonEmpty0.coq_NE_last rs0))) rs0))) __
-                      __ __;
-                   Prelude.Nothing -> Logic.coq_False_rec}}}) __) __};
-       Prelude.Nothing ->
-        case x of {
-         Prelude.Just r1 ->
-           (\_ -> (,) Prelude.Nothing (Prelude.Just (Build_IntervalDesc ib ie
-            (NonEmpty0.NE_Cons r rs0)))) __;
-         Prelude.Nothing -> Logic.coq_False_rec}}}}
-
-intervalSpan :: (NonEmpty0.NonEmpty Range.RangeDesc) -> Prelude.Int ->
-                Prelude.Int -> Prelude.Int ->
+intervalSpan :: ([] Range.RangeDesc) -> Prelude.Int -> Prelude.Int ->
+                Prelude.Int ->
                 ((,) (Prelude.Maybe IntervalDesc)
                 (Prelude.Maybe IntervalDesc))
 intervalSpan rs before ib ie =
-  intervalSpan_subproof rs before ib ie
+  let {f = \u -> (Prelude.<=) ((Prelude.succ) (Range.uloc u)) before} in
+  (\ns nc l -> case l of [x] -> ns x; (x:xs) -> nc x xs)
+    (\r ->
+    let {_top_assumption_ = Range.rangeSpan f ( r)} in
+    let {
+     _evar_0_ = \_top_assumption_0 ->
+      let {
+       _evar_0_ = \r0 _top_assumption_1 ->
+        let {
+         _evar_0_ = \r1 ->
+          let {
+           _evar_0_ = let {
+                       _evar_0_ = \_ _ -> (,) (Prelude.Just
+                        (Build_IntervalDesc (Range.rbeg ( r0))
+                        (Range.rend ( r0)) ((:[]) ( r0)))) (Prelude.Just
+                        (Build_IntervalDesc (Range.rbeg ( r1))
+                        (Range.rend ( r1)) ((:[]) ( r1))))}
+                      in
+                       _evar_0_}
+          in
+           _evar_0_ __ __}
+        in
+        let {
+         _evar_0_0 = \_ ->
+          let {
+           _evar_0_0 = \_ -> (,) (Prelude.Just (Build_IntervalDesc ib ie
+            ((:[]) r))) Prelude.Nothing}
+          in
+           _evar_0_0 __}
+        in
+        case _top_assumption_1 of {
+         Prelude.Just x -> (\_ -> _evar_0_ x);
+         Prelude.Nothing -> _evar_0_0}}
+      in
+      let {
+       _evar_0_0 = \_top_assumption_1 ->
+        let {
+         _evar_0_0 = \r1 ->
+          let {
+           _evar_0_0 = \_ -> (,) Prelude.Nothing (Prelude.Just
+            (Build_IntervalDesc ib ie ((:[]) r)))}
+          in
+           _evar_0_0 __}
+        in
+        let {_evar_0_1 = \_ -> Logic.coq_False_rec} in
+        case _top_assumption_1 of {
+         Prelude.Just x -> (\_ -> _evar_0_0 x);
+         Prelude.Nothing -> _evar_0_1}}
+      in
+      case _top_assumption_0 of {
+       Prelude.Just x -> _evar_0_ x;
+       Prelude.Nothing -> _evar_0_0}}
+    in
+    case _top_assumption_ of {
+     (,) x x0 -> _evar_0_ x x0 __})
+    (\r rs0 ->
+    let {_top_assumption_ = Range.rangeSpan f ( r)} in
+    let {
+     _evar_0_ = \_top_assumption_0 ->
+      let {
+       _evar_0_ = \r0 _top_assumption_1 ->
+        let {
+         _evar_0_ = \r1 ->
+          let {
+           _evar_0_ = \_ ->
+            let {
+             _evar_0_ = \_ _ ->
+              (Prelude.flip (Prelude.$)) __ (\_ -> (,) (Prelude.Just
+                (Build_IntervalDesc (Range.rbeg ( r0)) (Range.rend ( r0))
+                ((:[]) ( r0)))) (Prelude.Just (Build_IntervalDesc
+                (Range.rbeg ( r1)) (Range.rend ( (Prelude.last rs0))) ((:) r1
+                rs0))))}
+            in
+             _evar_0_ __ __}
+          in
+           _evar_0_ __}
+        in
+        let {
+         _evar_0_0 = \_ ->
+          let {
+           _evar_0_0 = \_ ->
+            let {
+             _evar_0_0 = \_ ->
+              let {
+               _top_assumption_2 = intervalSpan rs0 before
+                                     (Range.rbeg ( (Prelude.head rs0)))
+                                     (Range.rend ( (Prelude.last rs0)))}
+              in
+              let {
+               _evar_0_0 = \_top_assumption_3 ->
+                let {
+                 _evar_0_0 = \i1_1 _top_assumption_4 ->
+                  let {
+                   _evar_0_0 = \i1_2 ->
+                    case i1_1 of {
+                     Build_IntervalDesc ibeg0 iend0 rds0 ->
+                      let {
+                       _evar_0_0 = let {
+                                    _evar_0_0 = \_ _ ->
+                                     let {
+                                      _evar_0_0 = \_ ->
+                                       let {
+                                        _evar_0_0 = \_ ->
+                                         let {
+                                          _evar_0_0 = (Prelude.flip (Prelude.$))
+                                                        __ (\_ ->
+                                                        let {
+                                                         _evar_0_0 = \_ _ ->
+                                                          (,) (Prelude.Just
+                                                          (Build_IntervalDesc
+                                                          (Range.rbeg ( r))
+                                                          iend0 ((:) r
+                                                          rds0)))
+                                                          (Prelude.Just
+                                                          i1_2)}
+                                                        in
+                                                         _evar_0_0 __)}
+                                         in
+                                          _evar_0_0}
+                                       in
+                                        _evar_0_0 __}
+                                     in
+                                      _evar_0_0 __}
+                                   in
+                                    _evar_0_0}
+                      in
+                       _evar_0_0 __ __}}
+                  in
+                  let {
+                   _evar_0_1 = \_ ->
+                    let {
+                     _evar_0_1 = \_ _ _ -> (,) (Prelude.Just
+                      (Build_IntervalDesc (Range.rbeg ( r))
+                      (Range.rend ( (Prelude.last rs0))) ((:) r rs0)))
+                      Prelude.Nothing}
+                    in
+                     _evar_0_1 __}
+                  in
+                  case _top_assumption_4 of {
+                   Prelude.Just x -> (\_ _ -> _evar_0_0 x);
+                   Prelude.Nothing -> _evar_0_1}}
+                in
+                let {
+                 _evar_0_1 = \_top_assumption_4 ->
+                  let {
+                   _evar_0_1 = \i1_2 ->
+                    let {
+                     _evar_0_1 = \_ _ _ -> (,) (Prelude.Just
+                      (Build_IntervalDesc ib (Range.rend ( r)) ((:[]) r)))
+                      (Prelude.Just (Build_IntervalDesc
+                      (Range.rbeg ( (Prelude.head rs0)))
+                      (Range.rend ( (Prelude.last rs0))) rs0))}
+                    in
+                     _evar_0_1 __}
+                  in
+                  let {_evar_0_2 = \_ _ _ -> Logic.coq_False_rec} in
+                  case _top_assumption_4 of {
+                   Prelude.Just x -> (\_ -> _evar_0_1 x);
+                   Prelude.Nothing -> _evar_0_2}}
+                in
+                case _top_assumption_3 of {
+                 Prelude.Just x -> _evar_0_0 x;
+                 Prelude.Nothing -> _evar_0_1}}
+              in
+              case _top_assumption_2 of {
+               (,) x x0 -> _evar_0_0 x x0 __ __ __}}
+            in
+             _evar_0_0 __}
+          in
+           _evar_0_0 __}
+        in
+        case _top_assumption_1 of {
+         Prelude.Just x -> (\_ -> _evar_0_ x);
+         Prelude.Nothing -> _evar_0_0}}
+      in
+      let {
+       _evar_0_0 = \_top_assumption_1 ->
+        let {
+         _evar_0_0 = \r1 ->
+          let {
+           _evar_0_0 = \_ -> (,) Prelude.Nothing (Prelude.Just
+            (Build_IntervalDesc ib ie ((:) r rs0)))}
+          in
+           _evar_0_0 __}
+        in
+        let {_evar_0_1 = \_ -> Logic.coq_False_rec} in
+        case _top_assumption_1 of {
+         Prelude.Just x -> (\_ -> _evar_0_0 x);
+         Prelude.Nothing -> _evar_0_1}}
+      in
+      case _top_assumption_0 of {
+       Prelude.Just x -> _evar_0_ x;
+       Prelude.Nothing -> _evar_0_0}}
+    in
+    case _top_assumption_ of {
+     (,) x x0 -> _evar_0_ x x0 __})
+    rs
 
 splitInterval :: Prelude.Int -> IntervalDesc ->
                  ((,) IntervalDesc IntervalDesc)
