LinearScan/NonEmpty0.hs
@@ -2,56 +2,22 @@ module LinearScan.NonEmpty0 where
 
 import qualified Prelude
 import qualified Data.List
+import qualified Data.Ord
 import qualified Data.Functor.Identity
 import qualified LinearScan.Utils
 
-data NonEmpty a =
-   NE_Sing a
- | NE_Cons a (NonEmpty a)
-
-coq_NonEmpty_rect :: (a1 -> a2) -> (a1 -> (NonEmpty a1) -> a2 -> a2) ->
-                     (NonEmpty a1) -> a2
+coq_NonEmpty_rect :: (a1 -> a2) -> (a1 -> ([] a1) -> a2 -> a2) -> ([] 
+                     a1) -> a2
 coq_NonEmpty_rect f f0 n =
-  case n of {
-   NE_Sing y -> f y;
-   NE_Cons y n0 -> f0 y n0 (coq_NonEmpty_rect f f0 n0)}
+  (\ns nc l -> case l of [x] -> ns x; (x:xs) -> nc x xs)
+    (\y ->
+    f y)
+    (\y n0 ->
+    f0 y n0 (coq_NonEmpty_rect f f0 n0))
+    n
 
-coq_NonEmpty_rec :: (a1 -> a2) -> (a1 -> (NonEmpty a1) -> a2 -> a2) ->
-                    (NonEmpty a1) -> a2
+coq_NonEmpty_rec :: (a1 -> a2) -> (a1 -> ([] a1) -> a2 -> a2) -> ([] 
+                    a1) -> a2
 coq_NonEmpty_rec =
   coq_NonEmpty_rect
-
-coq_NE_length :: (NonEmpty a1) -> Prelude.Int
-coq_NE_length ne =
-  case ne of {
-   NE_Sing x -> (Prelude.succ) 0;
-   NE_Cons x xs -> (Prelude.+) ((Prelude.succ) 0) (coq_NE_length xs)}
-
-coq_NE_to_list :: (NonEmpty a1) -> [] a1
-coq_NE_to_list ne =
-  case ne of {
-   NE_Sing x -> (:) x [];
-   NE_Cons x xs -> (:) x (coq_NE_to_list xs)}
-
-coq_NE_head :: (NonEmpty a1) -> a1
-coq_NE_head ne =
-  case ne of {
-   NE_Sing x -> x;
-   NE_Cons x n -> x}
-
-coq_NE_last :: (NonEmpty a1) -> a1
-coq_NE_last ne =
-  case ne of {
-   NE_Sing x -> x;
-   NE_Cons x xs -> coq_NE_last xs}
-
-coq_NE_map :: (a1 -> a2) -> (NonEmpty a1) -> NonEmpty a2
-coq_NE_map f ne =
-  case ne of {
-   NE_Sing x -> NE_Sing (f x);
-   NE_Cons x xs -> NE_Cons (f x) (coq_NE_map f xs)}
-
-coq_NE_fold_left :: (a1 -> a2 -> a1) -> (NonEmpty a2) -> a1 -> a1
-coq_NE_fold_left f ne z =
-  Data.List.foldl' f z (coq_NE_to_list ne)
 
