Main.v
@@ -6,15 +6,15 @@
 
     https://www.usenix.org/legacy/events/vee05/full_papers/p132-wimmer.pdf
 *)
-Require Import Arith.
-Require Import Lib.
-Require Import NonEmpty.
-Require Import Blocks.
-Require Import Machine.
+Require Import LinearScan.Lib.
+Require Import LinearScan.NonEmpty.
+Require Import LinearScan.Blocks.
+Require Import LinearScan.Machine.
 
 Module MyMachine <: Machine.
 
 Definition maxReg := 32.
+Extract Constant maxReg => "32".
 
 Lemma registers_exist : (maxReg > 0).
 Proof. unfold maxReg. exact: ltn0Sn. Qed.
@@ -35,85 +35,36 @@ Set Extraction AccessOpaque.
 Extract Inductive Datatypes.nat => "Prelude.Int" ["0" "(Prelude.succ)"]
   "(\fO fS n -> if n Prelude.== 0 then fO () else fS (n Prelude.- 1))".
 
-Extract Inductive unit    => "()" [ "()" ].
-Extract Inductive bool    => "Prelude.Bool" ["Prelude.True" "Prelude.False"].
-Extract Inductive sumbool => "Prelude.Bool" ["Prelude.True" "Prelude.False"].
-Extract Inductive sum     => "Prelude.Either" [ "Prelude.Left" "Prelude.Right" ].
-Extract Inductive list    => "[]" ["[]" "(:)"].
-Extract Inductive prod    => "(,)" ["(,)"].
-Extract Inductive sigT    => "(,)" ["(,)"].
-Extract Inductive option  => "Prelude.Maybe" ["Prelude.Just" "Prelude.Nothing"].
-Extract Inductive sumor   => "Prelude.Maybe" ["Prelude.Just" "Prelude.Nothing"].
-
 Extract Inductive comparison =>
   "Prelude.Ordering" ["Prelude.LT" "Prelude.EQ" "Prelude.GT"].
 
-Extract Inlined Constant addn       => "(Prelude.+)".
-Extract Inlined Constant andb       => "(Prelude.&&)".
-Extract Inlined Constant app        => "(Prelude.++)".
-Extract Inlined Constant apply      => "(Prelude.$)".
-Extract Inlined Constant cat        => "(Prelude.++)".
-(* Extract Inlined Constant eq_op   => "(Prelude.==)". *)
-Extract Inlined Constant eqb        => "(Prelude.==)".
-Extract Inlined Constant eqn        => "(Prelude.==)".
-Extract Inlined Constant filter     => "Prelude.filter".
-Extract Inlined Constant foldl      => "Data.List.foldl'".
-Extract Inlined Constant foldr      => "Prelude.foldr".
-Extract Inlined Constant fst        => "Prelude.fst".
-(* Extract Inlined Constant id      => "Prelude.id". *)
-Extract Inlined Constant has        => "Data.List.any".
-Extract Inlined Constant length     => "Data.List.length".
-Extract Inlined Constant leq        => "(Prelude.<=)".
-Extract Inlined Constant map        => "Prelude.map".
-Extract Inlined Constant maxn       => "Prelude.max".
-Extract Inlined Constant minn       => "Prelude.min".
-Extract Inlined Constant minus      => "(Prelude.-)".
-Extract Inlined Constant mult       => "(Prelude.*)".
-Extract Inlined Constant negb       => "Prelude.not".
-Extract Inlined Constant orb        => "(Prelude.||)".
-Extract Inlined Constant plus       => "(Prelude.+)".
-Extract Inlined Constant tail_plus  => "(Prelude.+)".
-Extract Inlined Constant predn      => "Prelude.pred".
-Extract Inlined Constant proj1_sig  => "".
-Extract Inlined Constant projT1     => "Prelude.fst".
-Extract Inlined Constant rem        => "(Prelude.const Data.List.delete)".
-Extract Inlined Constant safe_hd    => "Prelude.head".
-Extract Inlined Constant size       => "Data.List.length".
-Extract Inlined Constant snd        => "Prelude.snd".
-Extract Inlined Constant subn       => "(Prelude.-)".
+Extract Inlined Constant apply   => "(Prelude.$)".
+Extract Inlined Constant safe_hd => "Prelude.head".
+Extract Inlined Constant sumlist => "Data.List.sum".
+Extract Inlined Constant lebf    => "Data.Ord.comparing".
+Extract Inlined Constant insert  => "Data.List.insertBy".
 
-Extraction Implicit eq_rect [ x y ].
-Extraction Implicit eq_rect_r [ x y ].
-Extraction Implicit eq_rec [ x y ].
-Extraction Implicit eq_rec_r [ x y ].
+Extract Inlined Constant Arith.Plus.tail_plus => "(Prelude.+)".
 
-Extract Inlined Constant eq_rect => "".
-Extract Inlined Constant eq_rect_r => "".
-Extract Inlined Constant eq_rec => "".
-Extract Inlined Constant eq_rec_r => "".
-
-Extraction Implicit funcomp [ u ].
-
-Extract Inlined Constant funcomp => "(Prelude..)".
-
-Extract Inductive simpl_fun => "(->)" [""].
-
-Extract Inlined Constant fun_of_simpl => "(Prelude.$)".
-Extract Inlined Constant SimplRel => "".
-Extract Inlined Constant ord_max => "".
-
-Extraction Implicit nat_of_ord [ n ].
 Extraction Implicit widen_id [ n ].
-Extraction Implicit widen_ord [ n m ].
 Extraction Implicit widen_fst [ n ].
 
-Extract Inlined Constant nat_of_ord => "".
 Extract Inlined Constant widen_id => "".
-Extract Inlined Constant widen_ord => "".
 Extract Inlined Constant widen_fst => "Prelude.id".
 
 Extract Inlined Constant List.destruct_list => "LinearScan.Utils.uncons".
-Extract Inlined Constant ssr_have => "(Prelude.flip (Prelude.$))".
+
+Extract Inductive NonEmpty => "[]" ["(:[])" "(:)"]
+  "(\ns nc l -> case l of [x] -> ns x; (x:xs) -> nc x xs)".
+
+Extract Inlined Constant NE_length  => "Prelude.length".
+Extract Inlined Constant NE_to_list => "".
+Extract Inlined Constant NE_head    => "Prelude.head".
+Extract Inlined Constant NE_last    => "Prelude.last".
+Extract Inlined Constant NE_map     => "Prelude.map".
+Extract Inlined Constant NE_foldl   => "Data.List.foldl'".
+
+Extract Inlined Constant list_membership => "Prelude.const".
 
 (* Avoid extracting this function, which has no computational value, but Coq
    insists on ignoring its opacity. *)
