Ssr.v
@@ -1,0 +1,77 @@
+Require Export Ssreflect.ssreflect.
+Require Export Ssreflect.ssrfun.
+Require Export Ssreflect.ssrbool.
+Require Export Ssreflect.eqtype.
+Require Export Ssreflect.seq.
+Require Export Ssreflect.ssrnat.
+Require Export Ssreflect.fintype.
+
+Extract Inductive unit    => "()" [ "()" ].
+Extract Inductive bool    => "Prelude.Bool" ["Prelude.True" "Prelude.False"].
+Extract Inductive sumbool => "Prelude.Bool" ["Prelude.True" "Prelude.False"].
+Extract Inductive sum     => "Prelude.Either" [ "Prelude.Left" "Prelude.Right" ].
+Extract Inductive list    => "[]" ["[]" "(:)"].
+Extract Inductive prod    => "(,)" ["(,)"].
+Extract Inductive sigT    => "(,)" ["(,)"].
+Extract Inductive option  => "Prelude.Maybe" ["Prelude.Just" "Prelude.Nothing"].
+Extract Inductive sumor   => "Prelude.Maybe" ["Prelude.Just" "Prelude.Nothing"].
+
+Extract Inductive ordinal => "Prelude.Int" [""].
+
+Extract Inlined Constant addn      => "(Prelude.+)".
+Extract Inlined Constant andb      => "(Prelude.&&)".
+Extract Inlined Constant app       => "(Prelude.++)".
+Extract Inlined Constant cat       => "(Prelude.++)".
+Extract Inlined Constant eqb       => "(Prelude.==)".
+Extract Inlined Constant eqn       => "(Prelude.==)".
+Extract Inlined Constant filter    => "Prelude.filter".
+Extract Inlined Constant foldl     => "Data.List.foldl'".
+Extract Inlined Constant foldr     => "Prelude.foldr".
+Extract Inlined Constant fst       => "Prelude.fst".
+Extract Inlined Constant has       => "Data.List.any".
+Extract Inlined Constant length    => "Data.List.length".
+Extract Inlined Constant leq       => "(Prelude.<=)".
+Extract Inlined Constant map       => "Prelude.map".
+Extract Inlined Constant maxn      => "Prelude.max".
+Extract Inlined Constant minn      => "Prelude.min".
+Extract Inlined Constant minus     => "(Prelude.-)".
+Extract Inlined Constant mult      => "(Prelude.*)".
+Extract Inlined Constant negb      => "Prelude.not".
+Extract Inlined Constant orb       => "(Prelude.||)".
+Extract Inlined Constant plus      => "(Prelude.+)".
+Extract Inlined Constant predn     => "Prelude.pred".
+Extract Inlined Constant proj1_sig => "".
+Extract Inlined Constant projT1    => "Prelude.fst".
+Extract Inlined Constant rem       => "(Prelude.const Data.List.delete)".
+Extract Inlined Constant size      => "Data.List.length".
+Extract Inlined Constant snd       => "Prelude.snd".
+Extract Inlined Constant subn      => "(Prelude.-)".
+
+Extraction Implicit eq_rect [ x y ].
+Extraction Implicit eq_rect_r [ x y ].
+Extraction Implicit eq_rec [ x y ].
+Extraction Implicit eq_rec_r [ x y ].
+
+Extract Inlined Constant eq_rect => "".
+Extract Inlined Constant eq_rect_r => "".
+Extract Inlined Constant eq_rec => "".
+Extract Inlined Constant eq_rec_r => "".
+
+Extraction Implicit funcomp [ u ].
+
+Extract Inlined Constant funcomp => "(Prelude..)".
+
+Extract Inductive simpl_fun => "(->)" [""].
+
+Extract Inlined Constant fun_of_simpl => "(Prelude.$)".
+Extract Inlined Constant SimplRel => "".
+
+Extract Inlined Constant ord_max => "".
+
+Extraction Implicit nat_of_ord [ n ].
+Extraction Implicit widen_ord [ n m ].
+
+Extract Inlined Constant nat_of_ord => "".
+Extract Inlined Constant widen_ord => "".
+
+Extract Inlined Constant ssr_have => "(Prelude.flip (Prelude.$))".
